Refactoring the GenRec library.

theories/Data/Lists.v
@@ -1,5 +1,6 @@
 Require Import Coq.Lists.List.
 Require Import ExtLib.Structures.Reducible.
+Require Import ExtLib.Data.Nat.
 
 Set Implicit Arguments.
 Set Strict Implicit.
@@ -41,3 +42,28 @@ Global Instance Monad_list : Monad list :=
 ; bind := fun _ _ x f =>
   List.fold_right (fun x acc => f x ++ acc) nil x
 }.
+
+
+Section list.
+  Inductive R_list_len {T} : list T -> list T -> Prop :=
+  | R_l_len : forall n m, length n < length m -> R_list_len n m.
+
+  Theorem wf_R_list_len T : well_founded (@R_list_len T).
+  Proof.
+    constructor. intros.
+    refine (@Fix _ _ wf_R_lt (fun n : nat => forall ls : list T, n = length ls -> Acc R_list_len ls)
+      (fun x rec ls pfls => Acc_intro _ _)
+      _ _ refl_equal).
+    refine (
+      match ls as ls return x = length ls -> forall z : list T, R_list_len z ls -> Acc R_list_len z with
+        | nil => fun (pfls : x = 0) z pf => _
+        | cons l ls => fun pfls z pf =>
+          rec _ (match pf in R_list_len xs ys return x = length ys -> R_nat_lt (length xs) x with
+                   | R_l_len n m pf' => fun pf_eq => match eq_sym pf_eq in _ = x return R_nat_lt (length n) x with
+                                                     | refl_equal => R_lt pf'
+                                                   end
+                 end pfls) _ eq_refl
+      end pfls).
+    clear - pf; abstract (inversion pf; subst; simpl in *; inversion H).
+  Defined.
+End list.
