theories/Data/Nat.v
@@ -1,0 +1,23 @@
+Set Implicit Arguments.
+Set Strict Implicit.
+
+Inductive R_nat_S : nat -> nat -> Prop :=
+| R_S : forall n, R_nat_S n (S n).
+
+Theorem wf_R_S : well_founded R_nat_S.
+Proof.
+  red; induction a; constructor; intros.
+    inversion H.
+    inversion H; subst; auto.
+Defined.
+
+Inductive R_nat_lt : nat -> nat -> Prop :=
+| R_lt : forall n m, n < m -> R_nat_lt n m.
+
+Theorem wf_R_lt : well_founded R_nat_lt.
+Proof.
+  red; induction a; constructor; intros.
+  { inversion H. exfalso. subst. inversion H0. }
+  { inversion H; clear H; subst. inversion H0; clear H0; subst; auto.
+    inversion IHa. eapply H. constructor. eapply H1. }
+Defined.
