theories/Data/Pair.v
@@ -1,0 +1,30 @@
+Set Implicit Arguments.
+Set Strict Implicit.
+
+Section PairWF.
+  Variables T U : Type.
+  Variable RT : T -> T -> Prop.
+  Variable RU : U -> U -> Prop.
+
+  Inductive R_pair : T * U -> T * U -> Prop :=
+  | L : forall l l' r r',
+    RT l l' -> R_pair (l,r) (l',r')
+  | R : forall l r r',
+    RU r r' -> R_pair (l,r) (l,r').
+
+  Hypothesis wf_RT : well_founded RT.
+  Hypothesis wf_RU : well_founded RU.
+
+  Theorem wf_R_pair : well_founded R_pair.
+  Proof.
+    red. intro x.
+    destruct x. generalize dependent u.
+    apply (well_founded_ind wf_RT (fun t => forall u : U, Acc R_pair (t, u))) .
+    do 2 intro.
+
+    apply (well_founded_ind wf_RU (fun u => Acc R_pair (x,u))). intros.
+    constructor. destruct y.
+    remember (t0,u). remember (x,x0). inversion 1; subst;
+    inversion H4; inversion H3; clear H4 H3; subst; eauto.
+  Defined.
+End PairWF.
